specs/verif_hmac_drbg_update.v
@@ -523,32 +523,42 @@ Proof.
 
   (* prove function post condition *)
   Exists K sep final_state_abs.
+  unfold hmac256drbgabs_hmac_drbg_update.
   unfold HMAC256_DRBG_functional_prog.HMAC256_DRBG_update.
+  destruct initial_state_abs.
   rewrite HMAC_DRBG_update_concrete_correct.
   Time entailer!. (* 29 *)
   {
-    remember (hmac256drbgabs_key final_state_abs, hmac256drbgabs_value final_state_abs) as final_key_value_pair.
-    replace (hmac256drbgabs_key final_state_abs) with (fst final_key_value_pair) by (subst final_key_value_pair; reflexivity).
-    replace (hmac256drbgabs_value final_state_abs) with (snd final_key_value_pair) by (subst final_key_value_pair; reflexivity).
-    rewrite H1.
+    rename H1 into Hupdate_rounds.
+    rename H6 into Hmetadata.
+    destruct final_state_abs; unfold hmac256drbgabs_metadata_same in Hmetadata.
+    destruct Hmetadata as [Hreseed_counter [Hentropy_len [Hpr Hrseed_interval]]]; subst.
     destruct contents; unfold HMAC_DRBG_update_concrete.
     {
-      (* contents = [] *)
-      simpl.
-      repeat split; try reflexivity.
-      apply hmac_common_lemmas.HMAC_Zlength.
-      apply hmac_common_lemmas.isbyte_hmac.
+      simpl in Hupdate_rounds; simpl.
+      clear - Hupdate_rounds.
+      replace (HMAC256 V (HMAC256 (V ++ [0]) key)) with V0.
+      replace (HMAC256 (V ++ [0]) key) with key0.
+      reflexivity.
+      change key0 with (fst (key0, V0)); rewrite Hupdate_rounds; reflexivity.
+      change V0 with (snd (key0, V0)); rewrite Hupdate_rounds; reflexivity.
     }
     {
-      repeat rewrite Zlength_map in *.
       destruct (eq_dec (Zlength (z :: contents)) 0) as [Zlength_eq | Zlength_neq].
       rewrite Zlength_cons, Zlength_correct in Zlength_eq; omega.
       destruct (eq_dec additional' nullval) as [additional_eq | additional_neq].
-      subst. inversion H10 as [isptr_null H']; inversion isptr_null.
-      simpl.
-      repeat split; try reflexivity.
-      apply hmac_common_lemmas.HMAC_Zlength.
-      apply hmac_common_lemmas.isbyte_hmac.
+      subst. repeat rewrite Zlength_map in H10; inversion H10 as [isptr_null H']; inversion isptr_null.
+      simpl in Hupdate_rounds; simpl.
+      replace (HMAC256 (HMAC256 V (HMAC256 (V ++ 0 :: z :: contents) key))
+        (HMAC256
+           (HMAC256 V (HMAC256 (V ++ 0 :: z :: contents) key) ++
+            1 :: z :: contents) (HMAC256 (V ++ 0 :: z :: contents) key))) with V0.
+      replace (HMAC256
+        (HMAC256 V (HMAC256 (V ++ 0 :: z :: contents) key) ++
+                 1 :: z :: contents) (HMAC256 (V ++ 0 :: z :: contents) key)) with key0.
+      reflexivity.
+      change key0 with (fst (key0, V0)); rewrite Hupdate_rounds; reflexivity.
+      change V0 with (snd (key0, V0)); rewrite Hupdate_rounds; reflexivity.
     }
   }
   unfold hmac_drbg_update_post.
